@prefix : <http://cdm.ovh/rst/typo/typo#> .
@prefix owl: <http://www.w3.org/2002/07/owl#> .
@prefix rdf: <http://www.w3.org/1999/02/22-rdf-syntax-ns#> .
@prefix xml: <http://www.w3.org/XML/1998/namespace> .
@prefix xsd: <http://www.w3.org/2001/XMLSchema#> .
@prefix list: <https://w3id.org/list#> .
@prefix rdfs: <http://www.w3.org/2000/01/rdf-schema#> .
@prefix dcterms: <http://purl.org/dc/terms/> .
@prefix rst-cons: <https://cdm.ovh/rst/cons/cons#> .
@prefix rst-typo: <https://cdm.ovh/rst/typo/typo#> .
@base <http://cdm.ovh/rst/typo/typo> .

<http://cdm.ovh/rst/typo/typo> rdf:type owl:Ontology ;
                                owl:versionIRI <http://cdm.ovh/rst/typo/0.2/typo> ;
                                dcterms:description """Defines:
* terms such as locomotive, wagon, trailer...
* features such as motored, passenger-carrying, freight-carrying...
* relations with rolling stock composition (vehicle, formation) that is the subject of another ontology."""@en ;
                                dcterms:license <ttps://interoperable-europe.ec.europa.eu/sites/default/files/custom-page/attachment/2020-03/EUPL-1.2%20EN.txt> ;
                                dcterms:title "Railway rolling stock typology"@en .

#################################################################
#    Annotation properties
#################################################################

###  http://purl.org/dc/terms/description
dcterms:description rdf:type owl:AnnotationProperty .


###  http://purl.org/dc/terms/license
dcterms:license rdf:type owl:AnnotationProperty .


###  http://purl.org/dc/terms/title
dcterms:title rdf:type owl:AnnotationProperty .


#################################################################
#    Datatypes
#################################################################

###  http://www.w3.org/2001/XMLSchema#boolean
xsd:boolean rdf:type rdfs:Datatype .


#################################################################
#    Data properties
#################################################################

###  http://cdm.ovh/rsm/rolling_stock/rolling_stock_typology#hasFixedConsist
<http://cdm.ovh/rsm/rolling_stock/rolling_stock_typology#hasFixedConsist> rdf:type owl:DatatypeProperty ,
                                                                                   owl:FunctionalProperty ;
                                                                          rdfs:domain rst-cons:Formation ;
                                                                          rdfs:range xsd:boolean ;
                                                                          rdfs:comment "Train formation, the consist of which cannot be changed while in operations as it would require interventions in a workshop."@en .


#################################################################
#    Classes
#################################################################

###  https://cdm.ovh/rst/cons/cons#Formation
rst-cons:Formation rdf:type owl:Class .


###  https://cdm.ovh/rst/cons/cons#Vehicle
rst-cons:Vehicle rdf:type owl:Class ;
                 rdfs:comment """Common definition in Directives 2016/797, 2016/798:
 a railway vehicle suitable for circulation on wheels on railway lines, with or without traction; a vehicle is composed of one or more structural and functional subsystems

ERA vocabulary 3.0.0: A specific vehicle or wagon able to operate over railway lines."""@en .


###  https://cdm.ovh/rst/typo/typo#Coach
rst-typo:Coach rdf:type owl:Class ;
               rdfs:subClassOf rst-cons:Vehicle ,
                               rst-typo:PassengerCarryingRollingStock ;
               rdfs:comment """TSI LOCPAS 2020:
a vehicle without traction in a fixed or variable formation capable of carrying passengers (by extension, requirements specified to apply to coaches in this TSI are deemed to apply also to restaurant cars, sleeping cars, couchettes cars, etc.)

Note: was \"passenger carriage\" in earlier versions."""@en .


###  https://cdm.ovh/rst/typo/typo#FreightCarryingRollingStock
rst-typo:FreightCarryingRollingStock rdf:type owl:Class ;
                                     rdfs:subClassOf rst-typo:RollingStockFeature ;
                                     rdfs:comment "Feature of Rolling stock: ability to carry freight, by design."@en .


###  https://cdm.ovh/rst/typo/typo#Locomotive
rst-typo:Locomotive rdf:type owl:Class ;
                    rdfs:subClassOf rst-cons:Vehicle ,
                                    rst-typo:MotoredRollingStock ;
                    rdfs:comment "Powered vehicle having a driving desk and can be used standalone (e.g. for shunting or ferrying movements), but is normally used for hauling other vehicles or formations."@en .


###  https://cdm.ovh/rst/typo/typo#MotorCar
rst-typo:MotorCar rdf:type owl:Class ;
                  rdfs:subClassOf rst-cons:Vehicle ,
                                  rst-typo:MotoredRollingStock ;
                  rdfs:comment """Powered vehicle that cannot be used standalone, as can be found in trainset (EMUs or DMUs).
May or may not carry passengers."""@en .


###  https://cdm.ovh/rst/typo/typo#MotoredRollingStock
rst-typo:MotoredRollingStock rdf:type owl:Class ;
                             rdfs:subClassOf rst-typo:RollingStockFeature ;
                             rdfs:comment "Feature of rolling stock that is able by design to exert tractive effort on wheels or (rarely) cogwheels."@en .


###  https://cdm.ovh/rst/typo/typo#OnTrackMachine
rst-typo:OnTrackMachine rdf:type owl:Class ;
                        rdfs:subClassOf rst-cons:Vehicle ,
                                        rst-typo:MotoredRollingStock ;
                        rdfs:comment "a motored railway vehicle used for infrastructure maintenance"@en .


###  https://cdm.ovh/rst/typo/typo#PassengerCarryingRollingStock
rst-typo:PassengerCarryingRollingStock rdf:type owl:Class ;
                                       rdfs:subClassOf rst-typo:RollingStockFeature ;
                                       rdfs:comment "Feature of Rolling stock: ability to carry freight, by design."@en .


###  https://cdm.ovh/rst/typo/typo#RailCar
rst-typo:RailCar rdf:type owl:Class ;
                 rdfs:subClassOf rst-cons:Vehicle ,
                                 rst-typo:MotoredRollingStock ,
                                 rst-typo:PassengerCarryingRollingStock ;
                 rdfs:comment """Wikipedia (12/3/2024): self-propelled railway vehicle designed to transport passengers.
Equiv. to FR: Autorail, DE: Schienenbus (narrower meaning: two axles only).
Note however the numerous variants and ambiguities."""@en .


###  https://cdm.ovh/rst/typo/typo#Rake
rst-typo:Rake rdf:type owl:Class ;
              rdfs:subClassOf rst-cons:Formation ;
              rdfs:comment """Any non-powered formation. Examples:
wagon rake;
(fixed consist) set of TGV trailers;
(fixed or variable consist) rake of coaches."""@en .


###  https://cdm.ovh/rst/typo/typo#RoadRailVehicle
rst-typo:RoadRailVehicle rdf:type owl:Class ;
                         rdfs:subClassOf rst-cons:Vehicle ,
                                         rst-typo:FreightCarryingRollingStock .


###  https://cdm.ovh/rst/typo/typo#RoadVehicleRake
rst-typo:RoadVehicleRake rdf:type owl:Class ;
                         rdfs:subClassOf rst-cons:Formation ;
                         rdfs:comment """From TSI WAG 2023, \"unit\", 3rd entry:
separate rail bogies connected to compatible road vehicle(s), the combination of which forms a rake of a rail compatible system."""@en .


###  https://cdm.ovh/rst/typo/typo#RollingStockFeature
rst-typo:RollingStockFeature rdf:type owl:Class .


###  https://cdm.ovh/rst/typo/typo#SlaveLocomotive
rst-typo:SlaveLocomotive rdf:type owl:Class ;
                         rdfs:subClassOf rst-cons:Vehicle ,
                                         rst-typo:MotoredRollingStock ;
                         rdfs:comment """Powered vehicle without driving desk, with energy possibly fed from master locomotive ( = subclass \"slug\").
Also called \"truck\" in France, e.g. TC61000.
Do not confuse with master/slave configuration of two normal locomotives (\"multiple working\" in the UK)."""@en .


###  https://cdm.ovh/rst/typo/typo#Trailer
rst-typo:Trailer rdf:type owl:Class ;
                 rdfs:subClassOf rst-cons:Vehicle ,
                                 rst-typo:PassengerCarryingRollingStock ;
                 rdfs:comment "non-traction, passenger-carrying vehicle that is part of a trainset or of a fixed-consist rake, such as TGV trailer or ICE3 trailer or Talgo trailer."@en .


###  https://cdm.ovh/rst/typo/typo#Trainset
rst-typo:Trainset rdf:type owl:Class ;
                  rdfs:subClassOf rst-cons:Formation ,
                                  rst-typo:MotoredRollingStock ;
                  rdfs:comment "TSI LOC&PAS, 2020: a fixed formation that can operate as a train; it is by definition not intended to be reconfigured, except within a workshop environment. It is composed of only motored or of motored and non-motored vehicles."@en .


###  https://cdm.ovh/rst/typo/typo#Van
rst-typo:Van rdf:type owl:Class ;
             rdfs:subClassOf rst-cons:Vehicle ,
                             rst-typo:FreightCarryingRollingStock ;
             rdfs:comment "TSI LOCPAS 2020: a vehicle without traction capable of carrying payload other than passengers, e.g. luggage or mail, intended to be integrated into a fixed or variable formation which is intended to transport passengers."@en .


###  https://cdm.ovh/rst/typo/typo#Wagon
rst-typo:Wagon rdf:type owl:Class ;
               rdfs:subClassOf rst-cons:Vehicle ,
                               rst-typo:FreightCarryingRollingStock ;
               rdfs:comment "A non-powered vehicle designed for carrying freight."@en .


###  Generated by the OWL API (version 4.5.29) https://github.com/owlcs/owlapi
